Verify clerk.GetConfig

src/program_proof/simplepb/config2_proof.v
@@ -953,7 +953,8 @@ Definition is_Clerk (ck:loc) γ : iProp Σ :=
   "#Hcls" ∷ readonly (ck ↦[config2.Clerk :: "cls"] (slice_val cls_sl)) ∗
   "#Hcls_sl" ∷ readonly (own_slice_small cls_sl (struct.ptrT Clerk) 1 cls) ∗
   "#Hrpc" ∷ ([∗ list] cl ∈ cls, ∃ srv, is_ReconnectingClient cl srv ∗ is_config_host srv γ) ∗
-  "%Hsz" ∷ ⌜ length cls = length config ⌝
+  "%Hsz" ∷ ⌜ length cls = length config ⌝ ∗
+  "%HszNonzero" ∷ ⌜ length config > 0 ⌝
 .
 
 Lemma wp_MakeClerk configHost γ:
@@ -1162,6 +1163,88 @@ Proof.
     wp_pures.
     wp_if_destruct.
     2:{ exfalso. done. }
+    iModIntro. iLeft.
+    iSplitR; first done.
+    iExists _. iFrame.
+  }
+Qed.
+
+Lemma wp_Clerk__GetConfig (ck:loc) γ Φ :
+  is_Clerk ck γ -∗
+  □ (∀ conf conf_sl, Pwf conf -∗ readonly (own_slice_small conf_sl uint64T 1 conf)
+                                 -∗ Φ (slice_val conf_sl)%V) -∗
+  WP config2.Clerk__GetConfig #ck {{ Φ }}
+.
+Proof.
+  iIntros "#Hck #HΦ".
+  wp_lam.
+  wp_apply wp_ref_of_zero.
+  { eauto. }
+  iIntros (reply_ptr) "Hreply".
+  wp_pures.
+  iAssert ( ∃ sl,
+      "Hreply" ∷ reply_ptr ↦[slice.T byteT] (slice_val sl)
+    )%I with "[-]" as "HH".
+  { rewrite zero_slice_val. iExists _; iFrame. }
+  wp_forBreak.
+  iNamed "HH".
+  wp_pures.
+  iNamed "Hck".
+  wp_apply (wp_RandomUint64).
+  iIntros (?) "_".
+  wp_loadField.
+  wp_apply wp_slice_len.
+  wp_pures.
+  wp_apply wp_NewSlice.
+  iIntros (?) "Hargs_sl".
+  iDestruct (own_slice_to_small with "Hargs_sl") as "Hargs_sl".
+  wp_loadField.
+
+  iMod (readonly_load with "Hcls_sl") as (?) "Hcls_sl2".
+  iDestruct (own_slice_small_sz with "Hcls_sl2") as %Hsl_sz.
+  set (idx:=(u64_instance.u64.(word.modu) r cls_sl.(Slice.sz))).
+  assert (int.nat idx < length cls) as Hlookup.
+  {
+    subst idx.
+    rewrite Hsl_sz.
+    rewrite word.unsigned_modu_nowrap; last lia.
+    { apply Z2Nat.inj_lt; auto using encoding.unsigned_64_nonneg.
+      { apply Z.mod_pos; lia. }
+      { apply Z_mod_lt; lia. }
+    }
+  }
+  apply list_lookup_lt in Hlookup as [? Hlookup].
+  wp_apply (wp_SliceGet with "[$Hcls_sl2]").
+  { done. }
+  iIntros "_".
+  iDestruct (big_sepL_lookup with "Hrpc") as (?) "#[Hcl_rpc Hhost]".
+  { exact Hlookup. }
+  iNamed "Hhost".
+  wp_apply (wp_ReconnectingClient__Call2 with "Hcl_rpc [] Hargs_sl Hreply").
+  { iDestruct "Hhost" as "(_ & $ & _)". }
+  { (* successful RPC *)
+    iModIntro.
+    iNext.
+    iIntros (?) "HP".
+    iIntros (?) "%Henc _".
+    iIntros (?) "Hrep Hreply_sl".
+    wp_pures.
+    iRight.
+    iModIntro. iSplitR; first done.
+    wp_pures.
+    wp_load.
+    wp_apply (Config.wp_Decode with "[$Hreply_sl //]").
+    iIntros (?) "Hconf".
+    wp_pures.
+    iApply ("HΦ" with "[$]").
+    iFrame.
+    done.
+  }
+  {
+    iIntros (?) "%Herr Hreply_sl Hrep".
+    wp_pures.
+    wp_if_destruct.
+    { exfalso. done. }
     iModIntro. iLeft.
     iSplitR; first done.
     iExists _. iFrame.
